

$$(1) \quad m(a + bX) = a + b \cdot m(X)$$

$$\text{We know: } m(X) = \frac{1}{N} \sum_{i=1}^N x_i$$

$$\Rightarrow m(a + bX) = \frac{1}{N} \sum_{i=1}^N (a + bx_i) = \frac{1}{N} \left(\sum_{i=1}^N a + b \sum_{i=1}^N x_i \right)$$

$$\text{we know } \sum_{i=1}^N a = Na$$

$$\begin{aligned} \therefore m(a + bX) &= \frac{1}{N} \left(aN + b \sum_{i=1}^N x_i \right) = a + b \left(\frac{1}{N} \sum_{i=1}^N x_i \right) \\ &= \underline{\underline{a + bm(X)}} \end{aligned}$$

$$(2) \quad \text{prove: } \text{cov}(X, a + bY) = b \text{cov}(X, Y)$$

$$\text{we know: } m(a + bY) = a + bm(Y)$$

$$\text{Cov}(X, a + bY) = \frac{1}{N} \sum_{i=1}^N (x_i - m(X)) ((a + by_i) - m(a + bY))$$

$$m(a + bY) = a + bm(Y)$$

$$\text{So, } (a + by_i) - (a + bm(Y)) = b(y_i - m(Y))$$

$$\therefore \text{cov}(X, a + bY) = \frac{1}{N} \sum_{i=1}^N (x_i - m(X)) \cdot b(y_i - m(Y))$$

$$\Rightarrow b \cdot \frac{1}{N} \sum_{i=1}^N (x_i - m(X)) (y_i - m(Y)) = \underline{\underline{b \text{cov}(X, Y)}}$$

$$\textcircled{3} \text{ cov}(a+bX, a+bX) = b^2 \text{cov}(X, X) \quad \& \text{ cov}(X, X) = s^2$$

→ Use Substitution, where $U = a + bX$, $U_i = a + bx_i$

$$\Rightarrow \text{cov}(U, U) = \frac{1}{N} \sum_{i=1}^N (U_i - m(U))(U_i - m(U))$$

$$m(U) = m(a + bX) = a + bm(X) \quad * \text{ proved in } \textcircled{1}$$

$$\begin{aligned} \text{then, } U_i - m(U) &= (a + bx_i) - (a + bm(X)) \\ &= b(x_i - m(X)) \end{aligned}$$

⇒ plugging in back into $\text{cov}(U, U)$

$$\rightarrow = \frac{1}{N} \sum_{i=1}^N b^2 (x_i - m(X))^2 = b^2 \cdot \underbrace{\frac{1}{N} \sum_{i=1}^N (x_i - m(X))(x_i - m(X))}_{\text{definition of cov}(X, X)}$$

$$\begin{aligned} \therefore \text{cov}(a+bX, a+bX) \\ &= \underline{b^2 \text{cov}(X, X)} \end{aligned}$$

$$\text{and since } s^2 = \frac{1}{N} \sum_{i=1}^N (x_i - m(X))^2$$

$$\text{cov}(a+bX, a+bX) = b^2 s^2$$

⑭ let \tilde{x} be the median, or median(x)

non-decreasing : if $x \geq x'$, then $g(x) \geq g(x')$

- If g is increasing & one-to-one on the sample, by applying g , it does not change which observation sits in the middle of ordered list, only ~~change~~ changes the value :

$$\text{median}(g(x)) = g(\text{median}(x))$$

"The transformed median(s) correspond to transforming the original median(s)."

\therefore Yes, monotonic, non-decreasing transformations carry medians to medians

Quantiles: by the same logic as before, a non-decreasing transformation preserves rank :

$$Q_p(g(x)) = g(Q_p(x)), \text{ non-uniqueness}$$

IQR:

$$IQR(X) = Q_{0.75}(X) - Q_{0.25}(X)$$

For non-decreasing g ,

$$IQR(g(x)) = Q_{0.75}(g(x)) - Q_{0.25}(g(x))$$

$$= g(Q_{0.75}(x)) - g(Q_{0.25}(x)) \quad \checkmark$$

$$\neq g(IQR(x)) \therefore \text{not does NOT apply}$$

Range:

$$\text{range}(x) = \max(x) - \min(x)$$

$$\text{range}(g(x)) = \max(g(x)) - \min(g(x))$$

$$= g(\max(x)) - g(\min(x))$$

$$\neq g(\text{range}(x)), \text{ a cannot distribute } g \text{ over}$$

DOES not Apply !!

however for a linear transformation: $g(x) = a + bx$
it becomes $b \text{range}(x)$

- ⑤ No, not generally, the mean uses arithmetic averaging where non-linear transformation do not commute w/ averaging

Example, let $X = \{0, 2\}$, $N = 2$, $g(x) = x^2$

↑
non-decreasing
from $[0, \infty)$

$$m(X) = \frac{0+2}{2} = 1, \quad g(m(X)) = 1^2 = 1$$

$$\text{but } m(g(x)) = \frac{0^2 + 2^2}{2} = \frac{0+4}{2} = 2$$

$$\therefore m(g(x)) \neq g(m(x))$$

however for linear $g(x) = a + bx$ then

$$m(g(x)) = m(a + bx) = a + b m(x) = g(m(x))$$

From Question 1, proof